Continue

src/Find_Urelems.thy
@@ -7,34 +7,335 @@ abbreviation "SEq \<equiv> Suc_Theory.Eq"
 abbreviation "SNEq \<equiv> Suc_Theory.NEq"
 
 fun constrs_term :: "('a pset_term \<Rightarrow> 'b) \<Rightarrow> 'a pset_term \<Rightarrow> 'b suc_atom list" where
-  "constrs_term _ (Var _) = []"
-| "constrs_term v (\<emptyset> n) = [SEq (SVar (v (\<emptyset> n))) (Succ n Zero)]"
-| "constrs_term v (t1 \<squnion>\<^sub>s t2) =
-    [SEq (SVar (v (t1 \<squnion>\<^sub>s t2))) (SVar (v t1)), SEq (SVar (v t1)) (SVar (v t2)), SNEq (SVar (v t1)) Zero]
-    @ constrs_term v t1 @ constrs_term v t2"
-| "constrs_term v (t1 \<sqinter>\<^sub>s t2) =
-    [SEq (SVar (v (t1 \<sqinter>\<^sub>s t2))) (SVar (v t1)), SEq (SVar (v t1)) (SVar (v t2)), SNEq (SVar (v t1)) Zero]
-    @ constrs_term v t1 @ constrs_term v t2"
-| "constrs_term v (t1 -\<^sub>s t2) =
-    [SEq (SVar (v (t1 -\<^sub>s t2))) (SVar (v t1)), SEq (SVar (v t1)) (SVar (v t2)), SNEq (SVar (v t1)) Zero]
-    @ constrs_term v t1 @ constrs_term v t2"
-| "constrs_term v (Single t) =
-    [SEq (SVar (v (Single t))) (Succ 1 (SVar (v t)))]
-    @ constrs_term v t"
+  "constrs_term n (Var x) = [SEq (SVar (n (Var x))) (SVar (n (Var x)))]"
+| "constrs_term n (\<emptyset> k) = [SEq (SVar (n (\<emptyset> k))) (Succ (Suc k) Zero)]"
+| "constrs_term n (t1 \<squnion>\<^sub>s t2) =
+    [SEq (SVar (n (t1 \<squnion>\<^sub>s t2))) (SVar (n t1)), SEq (SVar (n t1)) (SVar (n t2)), SNEq (SVar (n t1)) Zero]
+    @ constrs_term n t1 @ constrs_term n t2"
+| "constrs_term n (t1 \<sqinter>\<^sub>s t2) =
+    [SEq (SVar (n (t1 \<sqinter>\<^sub>s t2))) (SVar (n t1)), SEq (SVar (n t1)) (SVar (n t2)), SNEq (SVar (n t1)) Zero]
+    @ constrs_term n t1 @ constrs_term n t2"
+| "constrs_term n (t1 -\<^sub>s t2) =
+    [SEq (SVar (n (t1 -\<^sub>s t2))) (SVar (n t1)), SEq (SVar (n t1)) (SVar (n t2)), SNEq (SVar (n t1)) Zero]
+    @ constrs_term n t1 @ constrs_term n t2"
+| "constrs_term n (Single t) =
+    [SEq (SVar (n (Single t))) (Succ 1 (SVar (n t)))]
+    @ constrs_term n t"
       
 fun constrs_atom :: "('a pset_term \<Rightarrow> 'b) \<Rightarrow> 'a pset_atom \<Rightarrow> 'b suc_atom list" where
-  "constrs_atom v (t1 =\<^sub>s t2) =
-    [SEq (SVar (v t1)) (SVar (v t2))]
-    @ constrs_term v t1 @ constrs_term v t2"
-| "constrs_atom v (t1 \<in>\<^sub>s t2) =
-    [SEq (SVar (v t2)) (Succ 1 (SVar (v t1)))]
-    @ constrs_term v t1 @ constrs_term v t2"
+  "constrs_atom n (t1 =\<^sub>s t2) =
+    [SEq (SVar (n t1)) (SVar (n t2))]
+    @ constrs_term n t1 @ constrs_term n t2"
+| "constrs_atom n (t1 \<in>\<^sub>s t2) =
+    [SEq (SVar (n t2)) (Succ 1 (SVar (n t1)))]
+    @ constrs_term n t1 @ constrs_term n t2"
 
 fun constrs_fm :: "('a pset_term \<Rightarrow> 'b) \<Rightarrow> 'a pset_fm \<Rightarrow> 'b suc_atom list" where
-  "constrs_fm v (Atom a) = constrs_atom v a"
-| "constrs_fm v (And p q) = constrs_fm v p @ constrs_fm v q"
-| "constrs_fm v (Or p q) = constrs_fm v p @ constrs_fm v q"
-| "constrs_fm v (Neg p) = constrs_fm v p"
+  "constrs_fm n (Atom a) = constrs_atom n a"
+| "constrs_fm n (And p q) = constrs_fm n p @ constrs_fm n q"
+| "constrs_fm n (Or p q) = constrs_fm n p @ constrs_fm n q"
+| "constrs_fm n (Neg p) = constrs_fm n p"
+
+lemma is_Succ_normal_constrs_term:
+  "\<forall>a \<in> set (constrs_term n t). Suc_Theory.is_Eq a \<longrightarrow> is_Succ_normal a"
+  apply(induction t)
+       apply(auto)
+  done
+
+lemma is_Succ_normal_constrs_atom:
+  "\<forall>a \<in> set (constrs_atom n a). Suc_Theory.is_Eq a \<longrightarrow> is_Succ_normal a"
+  apply(cases a)
+  using is_Succ_normal_constrs_term apply(auto)
+  done
+
+lemma is_Succ_normal_constrs_fm:
+  "\<forall>a \<in> set (constrs_fm n \<phi>). Suc_Theory.is_Eq a \<longrightarrow> is_Succ_normal a"
+  apply(induction \<phi>)
+  using is_Succ_normal_constrs_atom apply(auto)
+  done
+
+lemma is_Var_Eq_Zero_if_is_NEq_constrs_term:
+  "\<forall>a \<in> set (constrs_term n t). Suc_Theory.is_NEq a \<longrightarrow> (\<exists>x. a = SNEq (SVar x) Zero)"
+  apply(induction t)
+       apply(auto)
+  done
+
+lemma is_Var_Eq_Zero_if_is_NEq_constrs_atom:
+  "\<forall>a \<in> set (constrs_atom n a). Suc_Theory.is_NEq a \<longrightarrow> (\<exists>x. a = SNEq (SVar x) Zero)"
+  apply(cases a)
+       using is_Var_Eq_Zero_if_is_NEq_constrs_term apply(auto)
+  done
+
+lemma is_Var_Eq_Zero_if_is_NEq_constrs_fm:
+  "\<forall>a \<in> set (constrs_fm n \<phi>). Suc_Theory.is_NEq a \<longrightarrow> (\<exists>x. a = SNEq (SVar x) Zero)"
+  apply(induction \<phi>)
+       using is_Var_Eq_Zero_if_is_NEq_constrs_atom apply(auto)
+  done
+
+lemma type_term_eq_Some_if_All_I_atom_constrs_term:
+  assumes "(\<forall>e \<in> set (constrs_term n t). Suc_Theory.I_atom v e)"
+  shows "type_term (\<lambda>x. v (n (Var x))) t = Some (v (n t))"
+  using assms
+  apply(induction t)
+       apply(auto simp: type_term.simps)
+  done
+
+lemma types_pset_atom_if_All_I_atom_constrs_atom:
+  assumes "(\<forall>e \<in> set (constrs_atom n a). Suc_Theory.I_atom v e)"
+  shows "(\<lambda>x. v (n (Var x))) \<turnstile> a"
+  using assms
+  by (cases a) (auto simp: types_pset_atom.simps type_term_eq_Some_if_All_I_atom_constrs_term)
+
+lemma types_pset_fm_if_All_I_atom_constrs_fm:
+  assumes "(\<forall>e \<in> set (constrs_fm n \<phi>). Suc_Theory.I_atom v e)"
+  shows "(\<lambda>x. v (n (Var x))) \<turnstile> \<phi>"
+  using assms
+  by (induction \<phi>)
+     (auto intro: types_fmI types_pset_atom_if_All_I_atom_constrs_atom)
+
+lemma I_atom_constrs_term_if_type_term_eq_Some:
+  assumes "inj_on n T" "subterms t \<subseteq> T"
+  assumes "type_term v t = Some k"
+  shows "(\<forall>e \<in> set (constrs_term n t).
+    Suc_Theory.I_atom (\<lambda>x. the (type_term v (inv_into T n x))) e)"
+  using assms
+  apply(induction t arbitrary: T k)
+       apply(auto simp: type_term.simps split: Option.bind_splits if_splits)
+  apply (metis inv_into_f_eq option.sel subset_iff subterms_refl)+
+  done
+
+lemma I_atom_constrs_atom_if_types_pset_atom:
+  assumes "inj_on n T" "subterms a \<subseteq> T"
+  assumes "v \<turnstile> a"
+  shows "(\<forall>e \<in> set (constrs_atom n a).
+    Suc_Theory.I_atom (\<lambda>x. the (type_term v (inv_into T n x))) e)"
+  using assms I_atom_constrs_term_if_type_term_eq_Some
+  by (cases a) (force simp: types_pset_atom.simps subsetD)+
+
+lemma I_atom_constrs_fm_if_types_pset_fm:
+  assumes "inj_on n T" "subterms \<phi> \<subseteq> T"
+  assumes "v \<turnstile> \<phi>"
+  shows "(\<forall>e \<in> set (constrs_fm n \<phi>).
+    Suc_Theory.I_atom (\<lambda>x. the (type_term v (inv_into T n x))) e)"
+  using assms
+  by (induction \<phi>)
+     (auto dest: types_fmD simp: I_atom_constrs_atom_if_types_pset_atom)
+
+
+lemma inv_into_f_eq_if_subs:
+  assumes "inj_on f B" "A \<subseteq> B" "y \<in> f ` A"
+  shows "inv_into B f y = inv_into A f y"
+  using assms inv_into_f_eq
+  by (metis f_inv_into_f inv_into_into subset_eq)
+
+lemma aux:
+  assumes "z \<in> \<Union>(set_suc_atom ` set (constrs_term n t))"
+  shows "z \<in> n ` subterms t"
+  using assms
+  apply(induction t)
+       apply(auto)
+  done
+
+lemma min_on_vars_if_min_on_set_suc_atom_constrs_term:
+  assumes "inj_on n (subterms t)"
+  assumes "\<And>v z. \<lbrakk> \<forall>a \<in> set (constrs_term n t). Suc_Theory.I_atom v a;
+                   z \<in> \<Union> (set_suc_atom ` set (constrs_term n t)) \<rbrakk>
+                 \<Longrightarrow> v_min z \<le> v z"
+  assumes "type_term (\<lambda>x. v_min (n (Var x))) t = Some lt" "type_term v t = Some lt'" "z \<in> vars t"
+  shows "v_min (n (Var z)) \<le> v z"
+proof -
+  define v' where "v' \<equiv> \<lambda>x. the (type_term v (inv_into (subterms t) n x))"
+  note I_atom_constrs_term_if_type_term_eq_Some[OF assms(1) _ assms(4)]
+  then have "\<forall>e \<in> set (constrs_term n t). Suc_Theory.I_atom v' e"
+    unfolding v'_def by blast
+  with assms(2)[OF this, unfolded v'_def] assms(1,3-) show ?thesis
+  proof(induction t arbitrary: lt lt')
+    case (Var x)
+    then show ?case
+      by (auto dest!: type_term_eq_SomeD(1))
+  next
+    case (Union t1 t2)
+    then have "subterms t1 \<subseteq> subterms (t1 \<squnion>\<^sub>s t2)" "subterms t2 \<subseteq> subterms (t1 \<squnion>\<^sub>s t2)"
+      by auto
+    note inv_into_simps =
+      this[THEN inv_into_f_eq_if_subs[OF \<open>inj_on n (subterms (t1 \<squnion>\<^sub>s t2))\<close> _ aux]]
+    with Union have "v_min z \<le> the (type_term v (inv_into (subterms t') n z))"
+      if "z \<in> \<Union> (set_suc_atom ` set (constrs_term n t'))" "t' \<in> {t1, t2}" for z t'
+      using that by simp metis
+    with Union show ?thesis
+      by (auto simp: inj_on_subset dest!: type_term_eq_SomeD(2))
+  next
+    case (Inter t1 t2)
+    then have "subterms t1 \<subseteq> subterms (t1 \<sqinter>\<^sub>s t2)" "subterms t2 \<subseteq> subterms (t1 \<sqinter>\<^sub>s t2)"
+      by auto
+    note inv_into_simps =
+      this[THEN inv_into_f_eq_if_subs[OF \<open>inj_on n (subterms (t1 \<sqinter>\<^sub>s t2))\<close> _ aux]]
+    with Inter have "v_min z \<le> the (type_term v (inv_into (subterms t') n z))"
+      if "z \<in> \<Union> (set_suc_atom ` set (constrs_term n t'))" "t' \<in> {t1, t2}" for z t'
+      using that by simp metis
+    with Inter show ?thesis
+      by (auto simp: inj_on_subset dest!: type_term_eq_SomeD(3))
+  next
+    case (Diff t1 t2)
+    then have "subterms t1 \<subseteq> subterms (t1 -\<^sub>s t2)" "subterms t2 \<subseteq> subterms (t1 -\<^sub>s t2)"
+      by auto
+    note inv_into_simps =
+      this[THEN inv_into_f_eq_if_subs[OF \<open>inj_on n (subterms (t1 -\<^sub>s t2))\<close> _ aux]]
+    with Diff have "v_min z \<le> the (type_term v (inv_into (subterms t') n z))"
+      if "z \<in> \<Union> (set_suc_atom ` set (constrs_term n t'))" "t' \<in> {t1, t2}" for z t'
+      using that by simp metis
+    with Diff show ?thesis
+      by (auto simp: inj_on_subset dest!: type_term_eq_SomeD(4))
+  next
+    case (Single t)
+    then have "subterms t \<subseteq> subterms (Single t)"
+      by auto
+    note inv_into_simps =
+      this[THEN inv_into_f_eq_if_subs[OF \<open>inj_on n (subterms (Single t))\<close> _ aux]]
+    with Single have "v_min z \<le> the (type_term v (inv_into (subterms t) n z))"
+      if "z \<in> \<Union> (set_suc_atom ` set (constrs_term n t))" for z
+      using that by simp metis
+    with Single show ?thesis
+      by (auto simp: inj_on_subset dest!: type_term_eq_SomeD(5))
+  qed simp
+qed
+
+lemma min_on_vars_if_min_on_set_suc_atom_constrs_atom:
+  fixes a :: "'a pset_atom"
+  assumes "inj_on n (subterms a)"
+  assumes "\<And>v z. \<lbrakk> \<forall>e \<in> set (constrs_atom n a). Suc_Theory.I_atom v e;
+                   z \<in> \<Union> (set_suc_atom ` set (constrs_atom n a)) \<rbrakk>
+                 \<Longrightarrow> v_min z \<le> v z"
+  assumes "(\<lambda>x. v_min (n (Var x))) \<turnstile> a" "v \<turnstile> a" "z \<in> vars a"
+  shows "v_min (n (Var z)) \<le> v z"
+proof(cases a)
+  case (Elem s t)
+  with assms have "inj_on n (subterms s)" "inj_on n (subterms t)"
+    by (auto simp: inj_on_Un)
+  note this[THEN min_on_vars_if_min_on_set_suc_atom_constrs_term]
+  moreover have "v_min z \<le> v z"
+    if "\<forall>e \<in> set (constrs_term n u). Suc_Theory.I_atom v e"
+       "z \<in> \<Union> (set_suc_atom ` set (constrs_term n u))"
+       "u \<in> {s, t}" for u v z
+    using that assms(2) Elem
+    apply(auto)
+  
+  with assms(3-) Elem show ?thesis sorry
+next
+  case (Equal x21 x22)
+  then show ?thesis sorry
+qed
+  using min_on_vars_if_min_on_set_suc_atom_constrs_term
+   apply(auto simp: types_pset_atom.simps )
+  sledgehammer
+
+lemma
+  assumes "inj_on n (subterms \<phi>)"
+  assumes "Suc_Theory.solve (Suc_Theory.elim_NEq_Zero (constrs_fm n \<phi>)) = Some ss"
+  shows "(\<lambda>x. Suc_Theory.assign ss (n (Var x))) \<turnstile> \<phi>"
+    and "\<And>v z. \<lbrakk> v \<turnstile> \<phi>; z \<in> vars \<phi> \<rbrakk> \<Longrightarrow> Suc_Theory.assign ss (n (Var z)) \<le> v z"
+proof -
+  note I_atom_assign_if_solve_elim_NEq_Zero_Some[OF _ _ assms(2)]
+  then have "\<forall>e \<in> set (constrs_fm n \<phi>). Suc_Theory.I_atom (Suc_Theory.assign ss) e"
+    using is_Succ_normal_constrs_fm is_Var_Eq_Zero_if_is_NEq_constrs_fm by blast
+  note types_pset_fm_if_All_I_atom_constrs_fm[OF this]
+  then show "(\<lambda>x. Suc_Theory.assign ss (n (Var x))) \<turnstile> \<phi>" .
+
+  note I_atom_assign_minimal_if_solve_elim_NEq_Zero_Some[OF _ _ assms(2)]
+  then have "Suc_Theory.assign ss z \<le> v z"
+    if "\<forall>a \<in> set (constrs_fm n \<phi>). Suc_Theory.I_atom v a"
+       "z \<in> \<Union> (set_suc_atom ` set (constrs_fm n \<phi>))" for v z
+    using that is_Succ_normal_constrs_fm is_Var_Eq_Zero_if_is_NEq_constrs_fm by blast
+
+  
+
+lemma aux2:
+  assumes "\<And>z. z \<in> vars t \<Longrightarrow> v_min z \<le> v z"
+  assumes "type_term v_min t = Some k'" "type_term v t = Some k"
+  shows "k' \<le> k"
+  using assms
+  apply(induction t arbitrary: k' k)
+       apply(auto simp: type_term.simps split: if_splits Option.bind_splits)
+  done
+
+lemma
+  assumes "inj_on n (subterms t)"
+  assumes "Suc_Theory.solve (Suc_Theory.elim_NEq_Zero (constrs_term n t)) = Some ss"
+  assumes "s \<in> subterms t"
+  assumes "type_term v t = Some kt"
+  shows "\<exists>k' k. type_term v s = Some k' \<and> type_term (\<lambda>x. Suc_Theory.assign ss (n (Var x))) s = Some k
+              \<and> k \<le> k'"
+proof -
+  let ?v' = "\<lambda>x. the (type_term v (inv_into (subterms t) n x))"
+  note All_I_atom_constrs_term_if_type_term_eq_Some[OF assms(1) _ assms(4)]
+  then have "(\<forall>e \<in> set (constrs_term n t). Suc_Theory.I_atom ?v' e)"
+    by blast  
+  note I_atom_assign_minimal_if_solve_elim_NEq_Zero_Some[OF _ _ assms(2) this]
+  then have "Suc_Theory.assign ss z \<le> ?v' z"
+    if "z \<in> \<Union> (set_suc_atom ` set (constrs_term n t))" for z
+    using is_Succ_normal_constrs_term is_Var_Eq_Zero_if_is_NEq_constrs_term
+    using that by blast
+  then have "Suc_Theory.assign ss (n (Var z)) \<le> v z"
+    if "z \<in> vars t" for z
+    using that \<open>inj_on n (subterms t)\<close> \<open>type_term v t = Some kt\<close>
+  proof(induction t arbitrary: kt)
+    case (Var x)
+    then show ?case by (simp add: type_term_eq_SomeD(1))
+  next
+    case (Union t1 t2)
+    have "subterms t1 \<subseteq> subterms (t1 \<squnion>\<^sub>s t2)" "subterms t2 \<subseteq> subterms (t1 \<squnion>\<^sub>s t2)"
+      by auto
+    note inv_into_f_eq_if_subs[OF \<open>inj_on n (subterms (t1 \<squnion>\<^sub>s t2))\<close> _ aux]
+    note this[OF \<open>subterms t1 \<subseteq> subterms (t1 \<squnion>\<^sub>s t2)\<close>] this[OF \<open>subterms t2 \<subseteq> subterms (t1 \<squnion>\<^sub>s t2)\<close>]
+    with Union have "Suc_Theory.assign ss z \<le> the (type_term v (inv_into (subterms t') n z))"
+      if "z \<in> \<Union> (set_suc_atom ` set (constrs_term n t'))" "t' \<in> {t1, t2}" for z t'
+      using that by auto metis+
+    with Union show ?case
+      by (auto simp: inj_on_Un dest: type_term_eq_SomeD)
+  next
+    case (Inter t1 t2)
+    have "subterms t1 \<subseteq> subterms (t1 \<sqinter>\<^sub>s t2)" "subterms t2 \<subseteq> subterms (t1 \<sqinter>\<^sub>s t2)"
+      by auto
+    note inv_into_f_eq_if_subs[OF \<open>inj_on n (subterms (t1 \<sqinter>\<^sub>s t2))\<close> _ aux]
+    note this[OF \<open>subterms t1 \<subseteq> subterms (t1 \<sqinter>\<^sub>s t2)\<close>] this[OF \<open>subterms t2 \<subseteq> subterms (t1 \<sqinter>\<^sub>s t2)\<close>]
+    with Inter have "Suc_Theory.assign ss z \<le> the (type_term v (inv_into (subterms t') n z))"
+      if "z \<in> \<Union> (set_suc_atom ` set (constrs_term n t'))" "t' \<in> {t1, t2}" for z t'
+      using that by auto metis+
+    with Inter show ?case
+      by (auto simp: inj_on_Un dest: type_term_eq_SomeD)
+  next
+    case (Diff t1 t2)
+    have "subterms t1 \<subseteq> subterms (t1 -\<^sub>s t2)" "subterms t2 \<subseteq> subterms (t1 -\<^sub>s t2)"
+      by auto
+    note inv_into_f_eq_if_subs[OF \<open>inj_on n (subterms (t1 -\<^sub>s t2))\<close> _ aux]
+    note this[OF \<open>subterms t1 \<subseteq> subterms (t1 -\<^sub>s t2)\<close>] this[OF \<open>subterms t2 \<subseteq> subterms (t1 -\<^sub>s t2)\<close>]
+    with Diff have "Suc_Theory.assign ss z \<le> the (type_term v (inv_into (subterms t') n z))"
+      if "z \<in> \<Union> (set_suc_atom ` set (constrs_term n t'))" "t' \<in> {t1, t2}" for z t'
+      using that by auto metis+
+    with Diff show ?case
+      by (auto simp: inj_on_Un dest: type_term_eq_SomeD)
+  next
+    case (Single t)
+    have "subterms t \<subseteq> subterms (Single t)"
+      by auto
+    note inv_into_f_eq_if_subs[OF \<open>inj_on n (subterms (Single t))\<close> this aux]
+    with Single have "Suc_Theory.assign ss z \<le> the (type_term v (inv_into (subterms t) n z))"
+      if "z \<in> \<Union> (set_suc_atom ` set (constrs_term n t))" for z
+      using that by auto metis+
+    with Single show ?case
+      by (auto simp: inj_on_Un dest: type_term_eq_SomeD)
+  qed simp
+  with \<open>s \<in> subterms t\<close> have "Suc_Theory.assign ss (n (Var z)) \<le> v z"
+    if "z \<in> vars s" for z
+    using that mem_vars_term_if_mem_subterms_term by metis
+  moreover obtain ks where "type_term (\<lambda>x. Suc_Theory.assign ss (n (Var x))) s = Some ks"
+    using Ex_type_term_assign_if_solve_constrs_term[OF assms(2)]
+    using type_term_if_mem_subterms[OF \<open>s \<in> subterms t\<close>] by blast
+  moreover obtain k's where "type_term v s = Some k's"
+    using type_term_if_mem_subterms[OF \<open>s \<in> subterms t\<close> assms(4)] by blast
+  ultimately show ?thesis
+    using aux2 by force
+qed
 
 hide_const (open) SVar SEq SNEq
 
